incr_cas/IncrementIAproof.v
@@ -1,77 +1,74 @@
 Require Import CRIS.
 Require Import SchHeader SchA SchTactics.
-Require Import ImpPrelude MemHeader MemA.
-From CRIS.incr_cas Require Import Header IncrementI IncrementA.
+Require Import ImpPrelude MemHeader MemA MemTactics.
+Require Import IncrementHeader IncrementI IncrementA.
 
 Module IncrementIA. Section IncrementIA.
-  Context `{CrisG: !crisG Γ Σ α β τ _S _I}.
-  Context `{MemG: !memG}.
-  Context `{SchG: !schG}.
+  Context `{!crisG Γ Σ α β τ _S _I, !memGS, !concGS, !schGS}.
+  Context (sp : specmap).
 
   Local Definition IstFull := (IstProd (IstSB IncrementA.t.(Mod.scopes) IstTrue) IstEq).
-  Local Definition MA := (IncrementA.t ★ MemA.t).
-  Local Definition MI := (IncrementI.t ★ MemA.t).
+  Local Definition MA := (IncrementA.t ★ (MemA.t sp)).
+  Local Definition MI := (IncrementI.t ★ (MemA.t sp)).
 
-  Lemma increment_simF : ISim.sim_fun open MA MI True%I IstFull (Some IncrementHdr.increment).
-  Proof using MemG SchG.
-    init_simF.
-    steps_l. destruct _q; ss. destruct _q; ss. destruct v; ss. inv G0. hss.
-    destruct _q0 as [blk ofs].
+  Lemma increment_simF : ISim.sim_fun open MA MI IstFull (Some IncrementHdr.increment).
+  Proof.
+    iStartSim.
+    steps_r. steps_l.
+    destruct (arg ↓) as [[|v [|v' l]]|]; step_l; ss.
+    destruct v as [|[blk ofs]|]; step_l; ss. steps_r.
 
-    steps_r.
-    sch_yield_rr.
-    steps_r. sch_yield_rr.
-    sch_yield_l.
-    norm_l. norm_r.
+    sch_yield_rr "IST". steps_r.
+    sch_yield_rr "IST". steps_r.
+    sch_yield_l. norm_l.
 
     iApply wsim_reset.
     iStopProof. revert st_src. combine_quant st_tgt.
     eapply wsim_coind.
-    iIntros (g' _ CIH [st_t st_s]) "%GG' /=".
+    iIntros (g' _ CIH [st_t st_s]) "IST /=".
     destruct_quant CIH.
 
-    unfold_iterC_l. unfold_iterC_r.
-    steps_l. steps_r.
-    sch_yield_rr.
-    Unshelve. all: try exact 0.
+    unfold_iterC_r. steps_r.
+    unfold_iterC_l. steps_l.
+    sch_yield_rr "IST".
 
     sch_yield_l. steps_l. rename _q into v.
 
-    steps_r. inline_r. force_r (blk, ofs, 1%Qp, Vint v). steps_r.
+    steps_r. inline_r. force_r (blk, ofs, 1%Qp, Vint v).
     forces_r. iFrame "ASM". iSplit; eauto.
-    steps_r. iDestruct "GRT" as "[[PT ->] ->]". hss_r. steps_r.
+    steps_r. iDestruct "GRT" as "[-> [↦ ->]]". rewrite Any.upcast_downcast /=. steps_r.
 
-    force_l false. steps_l. force_l; iFrame "PT". steps_l. sch_yield_l. steps_l.
+    force_l false. steps_l. force_l; iFrame "↦". steps_l. sch_yield_l. steps_l.
     unfold_iterC_l. steps_l.
 
-    sch_yield_rr. steps_r.
-    sch_yield_rr. steps_r.
+    sch_yield_rr "IST". steps_r.
+    sch_yield_rr "IST". steps_r.
 
     sch_yield_l. steps_l. rename _q into v'.
-    inline_r. force_r (_, _, _, _, _, _, _, _, _, _). forces_r. iFrame "ASM".
-    iSplitL ""; eauto.
-    { iSplit; eauto. iSplit; [iPureIntro; split; [refl|ss]|ss]. des_ifs. }
-    Unshelve. all: try exact 0; try exact 1%Qp; try exact (Vint 0).
+    iApply (wsim_mem_cas with "ASM"); [prove_inline_cond|ss|eauto| | | ].
+    { rewrite /MemA.compare_val; des_ifs. }
+    { instantiate (1:=emp%I); done. }
+    { iIntros "_"; iExists 1%Qp, 1%Qp, Vundef, Vundef; ss. }
+    iIntros "↦ _".
 
-    steps_r. iDestruct "GRT" as "[[-> [GRT _]] ->]". hss_r. steps_r.
-    destruct (dec v' v) as [?|Heq]; [subst; ss|ss].
-    { force_l true. steps_l. force_l; iFrame "GRT"; steps_l.
-      sch_yield_rr. steps_r.
-      sch_yield_rr; steps_r.
+    steps_r. rewrite Any.upcast_downcast /=. steps_r.
+    repeat case_bool_decide; subst; ss.
+    { force_l true. steps_l. force_l; iFrame "↦"; steps_l.
+      sch_yield_rr "IST". steps_r.
+      sch_yield_rr "IST"; steps_r.
       case_decide; [|ss].
       steps_r.
       sch_yield_l. steps_l. step. iSplit; done.
     }
     { force_l false.
-      forces_l. iFrame "GRT". steps_l.
-      sch_yield_rr; steps_r.
-      sch_yield_rr; steps_r.
+      forces_l. iFrame "↦". steps_l.
+      sch_yield_rr "IST"; steps_r.
+      sch_yield_rr "IST"; steps_r.
       case_decide; first clarify.
       steps_r.
       sch_yield_l. steps_l.
       iApply wsim_progress. iApply wsim_base.
       iIntros "?". iApply (CIH). iFrame.
     }
-    Unshelve. all: eauto.
   (*SLOW*)Qed.
 End IncrementIA. End IncrementIA.
