incr_faa/ClientI.v
@@ -1,9 +1,9 @@
 Require Import CRIS.
 Require Import ImpPrelude MemHeader SchHeader.
-From CRIS.incr_faa Require Import Header.
+Require Import FaaHeader.
 
 Module ClientI. Section ClientI.
-  Context {Σ : GRA}.
+  Context `{!crisG Γ Σ α β τ _S _I, !concGS}.
 
   Definition scopes : list string := [].
 
@@ -26,17 +26,16 @@ Module ClientI. Section ClientI.
       𝒴;;; '_ : unit <- trigger (IO "OUT" v);;
       𝒴;;; Ret (tt↑).
 
-  Definition fnsems : fnsems_type :=
-    [(Some IncrHdr.incr, (false, wmask_all, scopes, (None, cfunU (sfunU incr))));
-     (None,              (false, wmask_all, scopes, (None, main)))].
+  Definition fnsems : fnsemmap :=
+    {[Some IncrHdr.incr := Some (msk_real (msk_scp scopes msk_true), (None, cfunU (sfunU incr)));
+      None := Some (msk_real (msk_scp scopes msk_true), (None, main))]}.
 
   Program Definition smod : SMod.t := {|
     SMod.scopes := scopes;
     SMod.fnsems := fnsems;
-    SMod.initial_st := [];
+    SMod.initial_st := ∅;
   |}.
-  Solve All Obligations with prove_scope.
-  Next Obligation. prove_nodup. Qed.
+  Solve All Obligations with mod_tac.
 
-  Definition t : Mod.t := Seal.sealing CRIS (SMod.to_mod sp_none smod).
+  Definition t : Mod.t := SMod.to_mod ∅ smod.
 End ClientI. End ClientI.
