incr_faa/ClientIA.v
@@ -1,226 +1,203 @@
 Require Import CRIS.
-From CRIS.incr_faa Require Import Header ClientI ClientA FaaA.
-Require Import SchA MemA SchTactics.
+Require Export ClientI ClientA FaaA SchA MemA.
+Require Import SchTactics MemTactics.
 From iris Require Import frac_auth numbers.
+
+Require Import Common Mod ltac2_lib.
 
 (* Proof of refinement between ClientA.t and ClientI.t *)
 Module ClientIA. Section ClientIA.
   Import ClientA.
-  Context `{!crisG Γ Σ α β τ _S _I, !memG, !schG, !incrG}.
+  Context `{!crisG Γ Σ α β τ _S _I, !concGS, !memGS, !schGS, !incrG}.
 
-  Context (E : coPset) (q : Qp) (Hsub : ↑N_main ⊆ E).
-  Context (sp_user : spl_type).
-  Context (sp_s : string → option fspec).
-  Context (Hsch : sp_incl (SchAS.sp sp_user E q) sp_s).
-  Context (Hclient : spl_sub (ClientA.sp E q) sp_user).
+  Context (N : namespace).
+  Context (sp_user sp : specmap).
+  Context (Hclient : ClientA.sp N ⊆ sp_user).
+  Context (Hsch : SchA.sp sp_user (↑N) ⊆ sp).
 
-  Local Definition IstFull := (IstProd (IstSB (ClientA.t E q sp_s).(Mod.scopes) IstTrue) IstEq).
-  Local Definition init_cond := ClientA.init_cond E q.
-  Local Definition MA := (ClientA.t E q sp_s ★ MemA.t).
-  Local Definition MI := ((ClientI.t ★ FaaA.t) ★ MemA.t).
+  Local Definition IstFull := (IstProd (IstSB (ClientA.t N sp).(Mod.scopes) IstTrue) IstEq).
+  Local Definition MA := (ClientA.t N sp ★ MemA.t sp).
+  Local Definition MI := ((ClientI.t ★ FaaA.t) ★ MemA.t sp).
 
   Lemma f_spawnable γ v bofs :
-    SchAS.fspec_spawnable E q (incr_spec E q)
+    ⊢ SchA.fn_spawnable sp_user (IncrHdr.incr)
       (λ varg arg,
         ⌜varg = arg ∧ varg = ([Vptr bofs]↑↑)⌝
         ∗ counter γ (1/2) v
-        ∗ incr_inv 0 γ bofs)%I
+        ∗ incr_inv 0 N γ bofs)%I
       (λ vret ret,
         existT 0 ((⌜vret = ret ∧ vret = tt↑↑⌝ ∗ counter_syn γ (1/2) (v + 2))%SAT)).
-  Proof using.
-    rewrite /SchAS.fspec_spawnable /fspec_sch /fspec_virtual /precond /postcond /incr_spec /=.
-    ii; ss. eexists (x1, (bofs, v, γ)); split; red; ii.
-    - rewrite /precond /fspec_sch /fspec_simple /fspec_sch /precond /=.
-      iIntros "[W [% [-> [TID [% [-> [[-> ->] [C #INV]]]]]]]]". iFrame. eauto.
-    - rewrite /postcond /fspec_sch /fspec_simple /fspec_sch /postcond /=.
-      iIntros "[W [TID [[-> C] ->]]]". iFrame. iExists _; iSplitR; eauto.
-      iExists _; iSplitR; eauto. rewrite sl_red. iSplitR; eauto.
+  Proof using Hclient.
+    iExists _; iSplitL.
+    { simpl_sp. eauto. }
+    iApply SchA.fspec_sch_spawnable; first done.
+    iIntros "%P1 %Q1 [% [-> ->]]"; iExists _, _; iSplit; first (iPureIntro).
+    { exists (bofs, v, γ); split; ss. }
+    iIntros (varg arg) "[%va [%sarg [[% %] [% $]]]]"; des; clarify.
+    iIntros "!>"; iSplit; first done; iIntros "%% [[-> ->] ?] !>"; iExists _, _; iSplit; eauto.
+    solve_base_sl_red; iSplit; done.
   Qed.
 
-  Lemma incr_simF : ISim.sim_fun open MA MI init_cond IstFull (Some IncrHdr.incr).
-  Proof using Hsch Hclient Hsub.
-    init_simF.
+  Lemma incr_simF : ISim.sim_fun open MA MI IstFull (Some IncrHdr.incr).
+  Proof using Hsch Hclient.
+    iStartSim.
 
-    steps_l. iDestruct "ASM" as "[TID [[-> [C #INV]] ->]]". hss_l.
-    destruct _q5 as [b ofs]. rename _q1 into tid, _q4 into γ, _q6 into v.
+    steps_l. destruct _q as [[stid mtid] [[[blk ofs] v]]]; rename _q0 into varg.
+    iDestruct "ASM" as "[TID [[-> ->] [C #INV]]]". hss_l; hss_r.
 
-    steps_l. hss. steps_l.
-    steps_r. hss. steps_r.
-    rewrite /ClientI.incr /ClientA.incr /=. norm_l; norm_r.
+    steps_l. steps_r. hss_l. hss_r. steps_l. steps_r.
+    rewrite /ClientI.incr /ClientA.incr /=; steps_r. steps_l.
 
-    sch_yield_ir.
+    sch_yield_ir "IST" "TID".
 
     (* tgt inline - faa *)
-    steps_r; inline_r; steps_r.
-    hss_r; steps_r.
-    sch_yield_ir.
+    steps_r. inline_r. steps_r. hss_r. steps_r.
+    sch_yield_ir "IST" "TID".
 
-    rewrite /incr_inv.
-    iInv "INV" as "I" "IA".
-    iDestruct "I" as (x) "PT". iDestruct "PT" as "[PT CA]".
+    iInv "INV" as "[%x [PT CA]]" "IA".
 
     (* operational atomicity here *)
     forces_r; iFrame "PT"; steps_r.
 
     iMod (counter_incr 1 with "[C CA]") as "[C CA]"; first iFrame.
     iMod ("IA" with "[GRT CA]") as "_".
-    { iExists (x + 1)%Z; ss; iFrame. }
-    sch_yield_ir.
+    { iExists (x + 1)%Z; solve_base_sl_red; iFrame. }
+    sch_yield_ir "IST" "TID".
 
-    rewrite /incr_inv.
-    iInv "INV" as "I" "IA".
-    iDestruct "I" as (y) "PT". iDestruct "PT" as "[PT CA]".
+    iInv "INV" as "[%y [PT CA]]" "IA".
 
     (* operational atomicity here *)
     forces_r; iFrame "PT"; steps_r.
 
     iMod (counter_incr 1 with "[C CA]") as "[C CA]"; first iFrame.
     iMod ("IA" with "[GRT CA]") as "_".
-    { iExists (y + 1)%Z; ss; iFrame. }
-    sch_yield_ir.
+    { iExists (y + 1)%Z; solve_base_sl_red; iFrame. }
+    sch_yield_ir "IST" "TID".
 
     steps_r; hss_r; steps_r.
-    sch_yield_ir.
+    sch_yield_ir "IST" "TID".
     steps_r.
 
-    sch_yield_l; steps_l; forces_l; iFrame "TID".
+    sch_yield_l. steps_l. forces_l. iFrame "TID".
     iSplitL "C".
     { iFrame. replace (v + 1 + 1)%Z with (v + 2)%Z by lia. iFrame. eauto. }
-    steps_l. step; eauto.
+    steps_l. step. iFrame. done.
 (*SLOW*)Qed.
 
-  Lemma main_simF : ISim.sim_fun open MA MI init_cond IstFull None.
-  Proof using Hsch Hclient Hsub.
-    init_simF.
+  Lemma main_simF : ISim.sim_fun open MA MI IstFull None.
+  Proof using Hsch Hclient.
+    iStartSim.
 
-    steps_l. iDestruct "IST" as "[[-> ->] [W TID]]".
-    iApply (wsim_init_winv with "[W TID]"); iFrame "W"; hss.
-    steps_l.
+    steps_l. destruct _q as [[stid mtid] []]; s.
+    iDestruct "ASM" as "[TID ->]".
+    rewrite /main /ClientI.main.
 
     (* src/tgt yield *)
-    steps_r.
-    sch_yield_ir. iSplitL.
-    { iExists _, _, _, _; iSplit; eauto.
-      iSplit; eauto.
-      { iPureIntro; splits; ss; unfold_mod; ss. unfold_mod; ss. }
-    }
-    iIntros (??) "IST TID".
+    steps_r. steps_l.
+    sch_yield_ir "IST" "TID".
 
     (* tgt alloc *)
-    steps_r; inline_r.
-    force_r 1; forces_r; iSplit; eauto.
-    steps_r; iDestruct "GRT" as "[[%blk [-> [PT _]]] ->]"; hss_r; steps_r.
-    sch_yield_ir.
-    sch_yield_ir.
+    steps_r.
+    iApply wsim_mem_alloc. { prove_inline_cond. } { ss. } { ss. }
+    iIntros (blk) "[map _]". steps_r; hss_r; steps_r.
+    sch_yield_ir "IST" "TID". steps_r.
+    sch_yield_ir "IST" "TID". steps_r.
 
     (* tgt store *)
-    steps_r. inline_r.
-    force_r (_, _, _, _); forces_r; iFrame "PT"; iSplit; eauto.
-    steps_r. iDestruct "GRT" as "[[PT ->] ->]"; hss_r; steps_r.
-    sch_yield_ir.
+    store_r "map". steps_r. hss_r. steps_r.
+    sch_yield_ir "IST" "TID". steps_r.
     sch_yield_l. force_l (Vptr (blk, 0%Z)). steps_l. sch_yield_l. steps_l.
 
     (* spawn *)
     iMod (own_alloc ((●F 0%Z ⋅ ◯F{1} 0%Z))) as "[%γc [A F]]".
     { apply frac_auth_valid; ss. }
-    iMod (inv_alloc (ccounter_syn 0 γc (blk, 0%Z)) _ _ _ N_main with "[PT A]") as "#I"; eauto.
-    { rewrite sl_red. iExists (0%Z). iFrame. }
+    iMod (inv_alloc (ccounter_syn 0 γc (blk, 0%Z)) _ _ _ (N_main N) with "[map A]") as "#I"; eauto.
+    { apply nclose_subseteq. }
+    { solve_base_sl_red; iFrame. }
     iPoseProof (counter_op with "[F]") as "[F1 F2]".
     { rewrite -Qp.half_half -{2}(Z.add_0_r 0%Z). iApply "F". }
 
     iCombine "F1 I" as "F1". iCombine "F2 I" as "F2".
 
     (* src/tgt spawns *)
-    rewrite /Sch.spawn; steps_r; steps_l.
-    force_l (_, _, _); forces_l; iSplitL "F1 TID".
-    { iExists _; iSplit; eauto.
-      iFrame "TID"; iExists _, _, _; iSplit.
-      { iPureIntro; split; [done|split; [done|]].
-        eexists; split; last eapply f_spawnable.
-        eapply Hclient; ss.
-      }
-      ss; iFrame; iSplit; eauto.
+    rewrite /Sch.spawn; steps_r; steps_l. simpl_sp.
+    force_l (_, _); forces_l; iSplitL "F1".
+    { iExists _, _, _; iSplit; eauto.
+      iSplitR; first iApply f_spawnable.
+      iFrame; eauto.
     }
-    steps_l. call "IST".
-    steps_l. iDestruct "ASM" as "[% [-> [TID [% [[-> ->] TKN]]]]]". hss.
-    rename _q0 into tid1. steps_r. hss_r. steps_r.
-    sch_yield_ir.
+    steps_l. call "IST". clear_st. iIntros (ret ??) "IST".
+    steps_l. iDestruct "ASM" as "[% [[-> ->] Handle]]". hss_l. steps_l.
+    steps_r. hss_r. steps_r.
+    sch_yield_ir "IST" "TID".
     sch_yield_l.
 
-    rewrite /Sch.spawn; steps_r; steps_l.
-    force_l (_, _, _); forces_l; iSplitL "F2 TID".
-    { iExists _; iSplit; eauto.
-      iFrame "TID"; iExists _, _, _; iSplit.
-      { iPureIntro; split; [done|split; [done|]].
-        eexists; split; last eapply f_spawnable.
-        eapply Hclient; ss.
-      }
-      ss; iFrame; iSplit; eauto.
+    rewrite /Sch.spawn; steps_r; steps_l. simpl_sp.
+    force_l (_, _); forces_l; iSplitL "F2".
+    { iExists _, _, _; iSplit; eauto.
+      iSplitR; first iApply f_spawnable.
+      iFrame; eauto.
     }
-    steps_l. call "IST".
-    steps_l. iDestruct "ASM" as "[% [-> [TID [% [[-> ->] TKN2]]]]]". hss.
-    rename _q0 into tid2. steps_r. hss_r. steps_r.
-    sch_yield_ir.
+    steps_l. call "IST". clear_st. iIntros (ret ??) "IST".
+    steps_l. iDestruct "ASM" as "[% [[-> ->] Handle2]]". hss_l. steps_l.
+    steps_r. hss_r. steps_r.
+    sch_yield_ir "IST" "TID".
     sch_yield_l.
 
-    rewrite /Sch.join; steps_r; steps_l.
-    force_l (_, _, _); forces_l; iFrame "TKN TID"; iSplit; [iExists _; eauto|]. steps_l.
-    call "IST".
-    steps_l. iDestruct "ASM" as "[% [-> [% [% ASM]]]]"; hss.
-    iDestruct "ASM" as "[[% ->] [TID ASM]]". hss. rewrite sl_red. iDestruct "ASM" as "[[-> ->] Q]".
-    steps_r. hss_r. steps_r.
-    sch_yield_ir.
+    rewrite /Sch.join; steps_r; steps_l. simpl_sp.
+    force_l (_, _, _); forces_l. iFrame "TID Handle"; iSplit; [eauto|]. steps_l.
+    call "IST". clear_st. iIntros (ret ??) "IST".
+    steps_l. iDestruct "ASM" as "[TID [% [% [[-> ->] ASM]]]]".
+    solve_base_sl_red. iDestruct "ASM" as "[[-> ->] Q]".
+    hss_l. steps_l. steps_r. hss_r. steps_r.
+    sch_yield_ir "IST" "TID".
     sch_yield_l.
 
-    rewrite /Sch.join; steps_r; steps_l.
-    force_l (_, _, _); forces_l; iFrame "TKN2 TID"; iSplit; [iExists _; eauto|]. steps_l.
-    call "IST".
-    steps_l. iDestruct "ASM" as "[% [-> [% [% ASM]]]]"; hss.
-    iDestruct "ASM" as "[[% ->] [TID ASM]]". hss. rewrite sl_red. iDestruct "ASM" as "[[-> ->] Q2]".
-    steps_r. hss_r. steps_r.
-    sch_yield_ir.
+    rewrite /Sch.join; steps_r; steps_l. simpl_sp.
+    force_l (_, _, _); forces_l. iFrame "TID Handle2"; iSplit; [eauto|]. steps_l.
+    call "IST". clear_st. iIntros (ret ??) "IST".
+    steps_l. iDestruct "ASM" as "[TID [% [% [[-> ->] ASM]]]]".
+    solve_base_sl_red. iDestruct "ASM" as "[[-> ->] Q2]".
+    hss_l. steps_l. steps_r. hss_r. steps_r.
+    sch_yield_ir "IST" "TID".
 
-    iInv "I" as "INV" "INVA"; iDestruct "INV" as "[%x INV]".
-    iDestruct "INV" as "[PT C]".
+    iInv "I" as "[%x [PT C]]" "INVA".
     iCombine "C Q Q2" as "C" gives %[_ WF%frac_auth_agree]. inv WF; ss.
     iDestruct "C" as "[CA CF]".
 
-    steps_r. inline_r. steps_r. force_r (blk, 0%Z, 1%Qp, (Vint 4)). steps_r. forces_r.
-    iSplitL "PT"; eauto.
-    steps_r. iDestruct "GRT" as "[[PT ->] ->]". hss. steps_r.
+    steps_r. load_r "PT".  steps_r. hss_r. steps_r.
 
-    iMod ("INVA" with "[CA PT]") as "_".
-    { iExists 4; iFrame. }
+    iMod ("INVA" with "[CA PT]") as "_"; first solve_base_sl_red; iFrame.
 
-    sch_yield_ir. steps_r.
-    sch_yield_ir.
+    sch_yield_ir "IST" "TID". steps_r.
+    sch_yield_ir "IST" "TID". 
     sch_yield_l; steps_l.
 
     step.
     steps_l. steps_r.
-    sch_yield_ir.
-    sch_yield_l. steps_l.
-    step. eauto.
+    sch_yield_ir "IST" "TID".
+    sch_yield_l. steps_l. forces_l. iFrame "TID"; iSplit; eauto.
+    step. iFrame. done.
 (*SLOW*)Qed.
 
-  Lemma sim : ISim.t open MA MI init_cond IstFull.
-  Proof using Hsch Hclient Hsub.
+  Lemma sim : ISim.t open MA MI emp%I IstFull.
+  Proof using Hsch Hclient.
     init_sim.
     { eapply incr_simF. }
     { eapply main_simF. }
+    { iIntros "_"; iExists _, _, _, _; iSplit; eauto. }
   Qed.
 End ClientIA.
 
 Section ctxr.
-  Context `{!crisG Γ Σ α β τ _S _I, !memG, !schG, !incrG}.
+  Context `{!crisG Γ Σ α β τ _S _I, !concGS, !memGS, !schGS, !incrG}.
 
-  Definition ctxr (E : coPset) (q : Qp) (sp_s : string → option fspec) (sp_user : spl_type) :
-    ↑ClientA.N_main ⊆ E →
-    spl_sub (ClientA.sp E q) sp_user →
-    sp_incl (SchAS.sp sp_user E q) sp_s →
+  Definition ctxr (N : namespace) (sp_user sp : specmap) :
+    ClientA.sp N ⊆ sp_user →
+    (SchA.sp sp_user (↑N)) ⊆ sp →
     ctx_refines
-      (ClientA.t E q sp_s   ★ MemA.t, init_cond E q)
-      (ClientI.t            ★ FaaA.t ★ (MemA.t), emp%I).
+      (ClientA.t N sp ★ MemA.t sp, emp%I)
+      (ClientI.t      ★ FaaA.t ★ (MemA.t sp), emp%I).
   Proof using.
     etrans; cycle 1. { do 2 ctxr_rotate. ctxr_refl. }
     eset (GRP := ClientI.t ★ _).
