incr_faa/FaaI.v
@@ -1,28 +1,24 @@
 Require Import CRIS.
-Require Import ImpPrelude MemHeader MemA SchA SchTactics SchHeader.
-From CRIS.incr_faa Require Import Header.
+Require Import ImpPrelude MemHeader SchHeader.
+Require Import FaaHeader.
 
 Module FaaI. Section FaaI.
-  Context {Σ : GRA}.
+  Context `{!crisG Γ Σ α β τ _S _I, !concGS}.
 
   Definition scopes : list string := [].
 
   Definition faa2 : list val → itree crisE unit :=
-    λ arg,
-      𝒴;;; '_ : val <- MemHdr.faa arg;;
-      𝒴;;; '_ : val <- MemHdr.faa arg;;
-      𝒴;;; Ret tt.
+    λ arg, 𝒴;;; MemHdr.faa arg;;; 𝒴;;; MemHdr.faa arg;;; 𝒴;;; Ret tt.
 
-  Definition fnsems : fnsems_type :=
-    [(Some FaaHdr.faa2, (false, wmask_all, scopes, (None, cfunU faa2)))].
+  Definition fnsems : fnsemmap :=
+    {[Some FaaHdr.faa2 := Some (msk_scp scopes (msk_real msk_true), (None, cfunU faa2))]}.
 
   Program Definition smod : SMod.t := {|
     SMod.scopes := scopes;
     SMod.fnsems := fnsems;
-    SMod.initial_st := [];
+    SMod.initial_st := ∅;
   |}.
-  Solve All Obligations with prove_scope.
-  Next Obligation. prove_nodup. Qed.
+  Solve All Obligations with mod_tac.
 
-  Definition t : Mod.t := Seal.sealing CRIS (SMod.to_mod sp_none smod).
+  Definition t : Mod.t := SMod.to_mod ∅ smod.
 End FaaI. End FaaI.
