incr_faa/IncrAll.v
@@ -1,100 +1,68 @@
-Require Import CRIS Cancel.
+Require Import CRIS Cancel SMod CallFilter.
 Require Import MemI MemA MemIAproof ImpPrelude.
 Require Import SchHeader SchI SchA SchIAproof SchTactics.
-From CRIS.incr_faa Require Import Header ClientI ClientA ClientIA FaaI FaaA FaaIA.
+Require Import FaaHeader ClientI ClientA ClientIA FaaI FaaA FaaIA.
 
-Module ClientAll.
-  Import inv_instances.
-
-  Local Definition csl : string → bool := λ _, false.
-  Local Definition genv : GEnv.t := GEnv.unit.
-
-  Local Instance Γ : HRA := ##[invΓ; memΓ; schΓ; incrΓ].
-  Local Instance Σ : GRA := ##[Γ; invΣ; schΣ].
-
-  Definition irΓ : Γ :=
-    **[ir_invΓ; ir_memΓ csl genv; SchAS.ir_schΓ; *[None]].
-  Definition irΣ : Σ :=
-    **[irΓ; ir_invΣ; SchAS.ir_schΣ].
-
-  Lemma irΣ_valid : ✓ (irΣ ⋅ ir_own_admin).
-  Proof.
-    solve_ir_valid.
-    - apply ir_memRA_valid.
-    - apply SchAS.ir_tidRA_valid.
-    - apply SchAS.ir_threadsRA_valid.
-  Qed.
+Section ClientAux.
+  Context `{!crisG Γ Σ α β τ Hsub Hinv, !concGS, !memGS, !schGS, !incrG}.
+  Context (csl : string → bool) (genv : GEnv.t).
 
   (* source module *)
-  Local Definition sp_user_s : spl_type :=
-    ClientA.sp ⊤ 1%Qp.
-  Local Definition smod_src : SMod.t :=
-    (ClientA.smod ⊤ 1%Qp) ☆ (SchA.smod sp_user_s 1).
-  Local Definition mod_top : Mod.t := SMod.to_mod sp_none (SMod.cancel smod_src).
+  Local Definition sp_user_s : specmap := ClientA.sp nroot.
+  Local Definition smod_src : SMod.t := (ClientA.smod nroot) ☆ (SchA.smod sp_user_s ⊤).
+  Local Definition mod_top : Mod.t := SMod.to_mod ∅ (SMod.cancel smod_src).
   Local Definition mod_tgt : Mod.t := ClientI.t ★ FaaI.t ★ (MemI.t csl genv) ★ (SchI.t).
 
-  Local Definition sp : string → option fspec := sp_from smod_src.
+  Local Definition sp : specmap := SMod.conc_sp_from smod_src.
   Local Definition mod_src : Mod.t := SMod.to_mod sp smod_src.
 
-  (* Local Definition SchInSp0: sp_incl (SchAS.sp ⊤ (to_sp [])) (to_sp (SchAS.sp ⊤ (to_sp []))).
+  Local Definition SchInSp : (SchA.sp sp_user_s ⊤) ⊆ sp.
   Proof.
-    split; [|refl]. rewrite /SchAS.sp; unseal CRIS. prove_nodup.
-  Qed. *)
-  Local Definition SchInSp : sp_incl (SchAS.sp sp_user_s ⊤ 1%Qp) sp.
-  Proof.
-    rewrite /SchAS.sp; unseal CRIS.
-    split; [prove_nodup|].
-    intros ??; ss; des_ifs; des_sumbool; clarify; intros INV; inv INV;
-      rewrite /sp /smod_src /sp_from /= /to_sp /=; des_ifs; ss.
+    repeat try eapply insert_subseteq_l; last apply map_empty_subseteq;
+      rewrite lookup_insert_ne // lookup_kmap_Some; eexists (Some _); split; ss.
   Qed.
-  Local Definition UserInSp : sp_incl sp_user_s sp.
+  Local Definition UserInSp : sp_user_s ⊆ sp.
   Proof.
-    rewrite /sp_user_s /ClientA.sp /MemA.sp; unseal CRIS.
-    split; [prove_nodup|].
-    intros ??; ss; des_ifs; des_sumbool; clarify; intros INV; inv INV;
-      rewrite /sp /smod_src /sp_from /= /to_sp /=; des_ifs; ss.
+    repeat try eapply insert_subseteq_l; last apply map_empty_subseteq;
+      rewrite lookup_insert_ne // lookup_kmap_Some; eexists (Some _); split; ss.
   Qed.
-  Local Definition MainInSp : spl_sub (ClientA.sp ⊤ 1%Qp) sp_user_s.
-  Proof.
-    rewrite /spl_sub /sp_user_s /ClientA.sp /ClientA.incr_spec /=.
-    ii; rewrite ->eq_rel_dec_correct in *; des_ifs.
-  Qed.
-  (* Local Definition MemInSp : sp_incl MemA.sp sp.
-  Proof.
-    ii; rewrite /sp /SchAS.sp /MemA.sp /ClientA.sp; unseal CRIS; split; [prove_nodup|ii].
-    ss; des_ifs; rewrite ->eq_rel_dec_correct in *; des_ifs.
-  Qed. *)
+  Local Definition MainInSp : (ClientA.sp nroot) ⊆ sp_user_s.
+  Proof. by reflexivity. Qed.
 
   Local Definition init_cond : iProp Σ :=
-    MemA.init_cond csl genv ∗ SchA.init_cond ∗ ClientIA.ClientIA.init_cond ⊤ 1%Qp.
-  (* Local Definition main_fsp : fspec := ClientA.main_spec ⊤ 1%Qp. *)
+    MemA.init_cond csl genv ∗ SchA.init_cond.
 
   (* Apply cancellation to linked spec module *)
   Lemma cancel_src :
-    refines (mod_top, init_cond) (mod_src, init_cond).
+    refines
+      (mod_top, init_cond ∗ TID 0 ∗ YIELD 0 ∗ winv (⊤, ⊤) ∗ TidFrag 0 0 ∗ TIDAUTH 0 ∗ YIELDAUTH 1)%I
+      (mod_src, init_cond).
   Proof.
     eapply Cancel.cancellation.
-    { ii; des; subst; inv FIND; ss.
-      rewrite !eq_rel_dec_correct in H0; des_ifs.
+    { apply SMod.cancellable_add; r; rewrite /= /ClientA.fnsems /SchA.fnsems; mod_tac ss. }
+    { assert (Ht : SMod.conc_sp_from smod_src !! speckey_entry =
+        fsp_some (fspec_sch (↑nroot) fspec_trivial)); last (rewrite Ht; clear Ht).
+      { rewrite lookup_insert_ne // lookup_kmap_Some; exists None; split; ss. }
+       eexists _, _; splits.
+      { ss; exists (0, 0, tt); split; refl. }
+      { rewrite !nclose_nroot. iIntros "[$ [$ [$ $]]]"; ss. }
+      { unfold_pre_post. iIntros "% % [_ [_ $]]". }
     }
-    { econs; [refl|]; i; inv NS; des; inv H; des; inv H1;
-      rewrite !eq_rel_dec_correct in H2; des_ifs.
-    }
-    { econs; unfold_mod; ss; prove_nodup. }
   Qed.
 
   (* Refinement between spec/impl of whole program (linked module) *)
   Lemma src_tgt : refines (mod_src, init_cond) (mod_tgt, emp%I).
   Proof.
     eapply ctxr_refines.
-    rewrite /mod_src /mod_tgt /smod_src !add_interp_comm.
+    rewrite /mod_src /mod_tgt /smod_src.
 
     (* abstraction of Sch *)
     etrans; cycle 1.
     { do 3 ctxr_drop.
-      eapply main_adequacy, SchIA.sim.
+      eapply SchIA.ctxr.
       - apply SchInSp.
       - apply UserInSp.
+      - rewrite dom_insert elem_of_union; left; apply elem_of_singleton; ss.
     }
 
     (* abstraction of Mem *)
@@ -113,10 +81,9 @@ Module ClientAll.
     (* abstraction of Incr *)
     etrans; cycle 1.
     { ctxr_drop.
-      eapply ClientIA.ctxr.
-      - instantiate (1:=⊤). set_solver.
+      eapply ClientIA.ctxr; cycle 2.
       - apply MainInSp.
-      - apply SchInSp.
+      - rewrite nclose_nroot. apply SchInSp.
     }
 
     etrans; cycle 1.
@@ -124,20 +91,18 @@ Module ClientAll.
 
     (* elimination of mem *)
     etrans; cycle 1.
-    { do 2 ctxr_rotate. do 2 ctxr_drop. eapply CFilter.elim_module. }
+    { do 2 ctxr_rotate. do 2 ctxr_drop. eapply elim_module. }
     rewrite -mod_add_empty_r.
 
     rewrite /SchIAproof.SchIA.SchAMod.
     rewrite /SchA.t /ClientA.t /MemA.t.
     unseal CRIS.
     ctxr_rotate.
-    
-    eapply ctxr_cond_strengthen.
-    { iIntros "[? [? ?]]". iFrame. }
+    rewrite SMod.to_mod_add /init_cond //.
   (*SLOW*)Qed.
 
   Lemma top_tgt :
-    refines (mod_top, init_cond)
+    refines (mod_top, init_cond ∗ TID 0 ∗ YIELD 0 ∗ winv (⊤, ⊤) ∗ TidFrag 0 0 ∗ TIDAUTH 0 ∗ YIELDAUTH 1)%I
             (mod_tgt, emp%I).
   Proof.
     etrans.
@@ -145,38 +110,59 @@ Module ClientAll.
     { eapply src_tgt. }
   Qed.
 
-  Lemma tgt_wf:
-    Mod.wf mod_tgt.
+  Lemma tgt_wf : Mod.wf mod_tgt.
   Proof.
-    rewrite /mod_tgt /ClientI.t /FaaI.t /MemI.t /SchI.t; unseal CRIS; prove_nodup.
-  Qed.
-
-  Lemma init_cond_valid:
-    ∃ rs, ✓ rs ∧ (Own rs ⊢ |==> init_cond).
-  Proof.
-    exists (irΣ ⋅ ir_own_admin). split.
-    - apply irΣ_valid.
-    - simplify_res.
-      { rewrite make_own_admin; iFrame.
-        erewrite SchAS.tid_admin_none.
-        iMod (SchAS.tid_admin_none_split 0 with "H22") as "[TA TU]".
-        iSplitR "TA TU".
-        - rewrite /init_cond. iAssert (mem_init csl genv) with "[H24]" as "[$ _]". eauto. done.
-        - unfold_pre_post; iFrame. done.
+    rewrite /mod_tgt; eapply Mod.add_wf.
+    { econs; eauto; [mod_tac|prove_nodup]. }
+    { eapply Mod.add_wf.
+      { econs; eauto; [mod_tac|prove_nodup]. }
+      { eapply Mod.add_wf.
+        { econs; eauto; [mod_tac|prove_nodup]. }
+        { econs; eauto; [mod_tac|prove_nodup]. }
+        { set_solver. }
+        { prove_nodup; set_solver. }
       }
-      all: solve_res.
+      { rewrite Mod.dom_fnsems_add; set_solver. }
+      { prove_nodup; set_solver. }
+    }
+    { rewrite !Mod.dom_fnsems_add; set_solver. }
+    { prove_nodup; set_solver. }
   Qed.
+End ClientAux.
+
+Module ClientAll. 
+  Import inv_instances.
+
+  Local Definition csl : string → bool := λ _, false.
+  Local Definition genv : GEnv.t := GEnv.unit.
+
+  Local Instance Γ : HRA := ##[invΓ; concΓ; memΓ; newschΓ; incrΓ].
+  Local Instance Σ : GRA := ##[Γ; invΣ; newschΣ].
 
   Theorem behavioral_refinement :
-    ∃ src_res tgt_res, refines_lmod
+    ∃ β τ (Hinv : invGS Γ Σ α) (_ : crisG Γ Σ α β τ _ Hinv) (_ : concGS) (_ : schGS) (_ : memGS)
+      src_res tgt_res,
+    refines_lmod
       (Mod.to_lmod mod_top src_res)
-      (Mod.to_lmod mod_tgt tgt_res).
+      (Mod.to_lmod (mod_tgt csl genv) tgt_res).
   Proof.
-    move: (top_tgt)=>H; rewrite /refines in H; des; ss.
-    hexploit H; eauto using tgt_wf. clear H; intros [WF H].
-    assert (IV:= init_cond_valid). des.
-    destruct (H rs); des; et.
-    rewrite IV0 /init_cond /ClientIA.ClientIA.init_cond /ClientA.init_cond.
-    rewrite {1}winv_split_empty. iIntros ">[? [? [[? ?] ?]]]". iFrame. et.
+    apply own_admin_soundness.
+    iMod winv_alloc as "[% [% [% [% ?]]]]"; iExists _, _, _, _.
+    iMod conc_alloc as "[% ?]"; iExists _.
+    iMod sch_alloc as "[% ?]"; iExists _.
+    iMod (mem_alloc csl genv) as "[% ?]"; iExists _.
+    pose proof (top_tgt csl genv) as Href.
+    iStopProof. eapply entails_pointwise; iIntros (res Hres) "R".
+    iPoseProof (Own_valid with "R") as "%".
+    rewrite /refines in Href; hexploit Href; eauto using tgt_wf.
+    clear Href; intros [? Href].
+    iPureIntro; hexploit (Href res); eauto.
+    { rewrite Hres; iIntros "[W [[$ [$ [$ $]]] [[$ $] [$ _]]]]".
+      rewrite {1}winv_split_empty comm //.
+    }
+    intros [rt ?].
+    exists res, rt; by des.
   (*SLOW*)Qed.
 End ClientAll.
+
+(* Print Assumptions ClientAll.behavioral_refinement. *)
