spinlock_na/LockA.v
@@ -1,5 +1,5 @@
 Require Import CRIS.
-From CRIS.spinlock_na Require Import Header.
+Require Import LockHeader.
 Require Import ImpPrelude MemHeader MemA.
 Require Import SchHeader SchA.
 From iris Require Import excl.
@@ -9,7 +9,6 @@ From iris Require Import excl.
 (* Resource algebra *)
 (* Structure of the resource algebra definition is similar to that of iris,
   but few differences exist. *)
-(* HRAs are structs similar to GRAs, but for RAs that sProps can own. *)
 Section RA.
   Context `{!crisG Γ Σ α β τ _S _I}.
   
@@ -17,24 +16,14 @@ Section RA.
     spinlock_inG :: inG (exclR unitO) Γ;
   }.
   Definition spinlockΓ : HRA := #[exclR unitO].
-  (* Be sure to annotate Γ as HRA, or tc search may not work properly. *)
   Global Instance subG_spinlockG : subG spinlockΓ Γ → spinlockG.
   Proof. solve_inG. Defined.
-  (* Be sure to add these two instances to hint database so that we can resolve inG instances
-    in the cancellation phase. *)
 End RA.
-Hint Unfold subG_spinlockG spinlock_inG : GRA_index.
 
 (* Spec definition *)
 (* Define 1) initial resource 2) function specs 3) sp here. *)
-Module LockAS. Section LockAS.
-  Context `{_crisG: !crisG Γ Σ α β τ _S _I}.
-  Context `{_memG: !memG}.
-  Context `{_schG: !schG}.
-  Context `{_spinlockG: !spinlockG}.
-
-  (* Initial resource *)
-  Definition ir : spinlockΓ := *[None].
+Module LockA. Section LockA.
+  Context `{!crisG Γ Σ α β τ _S _I, !concGS, !memGS, !schGS, !spinlockG}.
 
   Definition N_SpinLockA := nroot .@ "spin_lock".
 
@@ -48,24 +37,24 @@ Module LockAS. Section LockAS.
     ∃ bofs, ⌜val = Vptr bofs⌝ ∗ inv n N_SpinLockA (lock_inv bofs P γ).
 
   (* Function specs *)
-  Definition newlock_spec E q : fspec :=
-    fspec_winv E (fspec_sch q
+  Definition newlock_spec E : fspec :=
+    (fspec_sch E
       (fspec_simple (X := {n & GTerm.t n})
         (λ '(existT n P),
           ((λ _, ⟦P⟧),
           (λ ret, ∃ val γ, ⌜ret = val↑⌝ ∗ is_lock γ val P))
       ))%I).
 
-  Definition acquire_spec E q : fspec :=
-    fspec_winv E (fspec_sch q
+  Definition acquire_spec E : fspec :=
+    (fspec_sch E
       (fspec_simple (X := gname * val * {n & GTerm.t n})
         (λ '(γ, val, P),
           ((λ arg, ⌜arg = [val]↑⌝ ∗ is_lock γ val (projT2 P)),
           (λ ret, ⌜ret = Vundef↑⌝ ∗ ⟦token (projT1 P) γ⟧ ∗ ⟦projT2 P⟧))
       )))%I.
 
-  Definition release_spec E q : fspec :=
-    fspec_winv E (fspec_sch q
+  Definition release_spec E : fspec :=
+    (fspec_sch E
       (fspec_simple (X := gname * val * {n & GTerm.t n})
         (λ '(γ, val, P),
           ((λ arg, ⌜arg = [val]↑⌝
@@ -75,46 +64,37 @@ Module LockAS. Section LockAS.
           (λ ret, ⌜ret = Vundef↑⌝))
       )))%I.
 
-  Definition sp E q : spl_type :=
-    [(Some SpinLockHdr.newlock, Some (newlock_spec E q));
-     (Some SpinLockHdr.acquire, Some (acquire_spec E q));
-     (Some SpinLockHdr.release, Some (release_spec E q))].
-End LockAS. End LockAS.
+  Definition sp E : specmap :=
+    {[speckey_fn SpinLockHdr.newlock := fspec_to_rel (newlock_spec E);
+      speckey_fn SpinLockHdr.acquire := fspec_to_rel (acquire_spec E);
+      speckey_fn SpinLockHdr.release := fspec_to_rel (release_spec E)]}.
 
-(* Module definition *)
-(* Define three components for a module:
-  1) scope
-  2) code (via itree)
-  3) initial state (via Any.t)
-*)
-Module SpinLockA. Section SpinLockA.
-  Context `{_crisG: !crisG Γ Σ α β τ _S _I}.
-  Context `{_memG: !memG}.
-  Context `{_schG: !schG}.
-  Context `{_spinlockG: !spinlockG}.
-
+  (* Module definition *)
+  (* Define three components for a module:
+    1) scope
+    2) code (via itree)
+    3) initial state (via Any.t)
+  *)
   Definition scopes : list string := [].
 
   Definition newlock : list val → itree crisE val :=
     λ _, 𝒴;;; trigger (Choose val).
-
   Definition acquire : list val → itree crisE val :=
     λ _, 𝒴;;; Ret Vundef.
   Definition release : list val → itree crisE val :=
     λ _, 𝒴;;; Ret Vundef.
 
-  Definition fnsems E q : fnsems_type :=
-    [(Some SpinLockHdr.newlock, (true, wmask_all, scopes, (Some (LockAS.newlock_spec E q), cfunU newlock)));
-     (Some SpinLockHdr.acquire, (true, wmask_all, scopes, (Some (LockAS.acquire_spec E q), cfunU acquire)));
-     (Some SpinLockHdr.release, (true, wmask_all, scopes, (Some (LockAS.release_spec E q), cfunU release)))].
+  Definition fnsems (E : coPset) : fnsemmap :=
+    {[Some SpinLockHdr.newlock := Some (msk_scp scopes msk_true, (fsp_some (newlock_spec E), cfunU newlock));
+      Some SpinLockHdr.acquire := Some (msk_scp scopes msk_true, (fsp_some (acquire_spec E), cfunU acquire));
+      Some SpinLockHdr.release := Some (msk_scp scopes msk_true, (fsp_some (release_spec E), cfunU release))]}.
 
-  Program Definition smod E q : SMod.t := {|
-    SMod.scopes := [];
-    SMod.fnsems := fnsems E q;
-    SMod.initial_st := []
+  Program Definition smod E : SMod.t := {|
+    SMod.scopes := scopes;
+    SMod.fnsems := fnsems E;
+    SMod.initial_st := ∅
   |}.
-  Solve All Obligations with prove_scope.
-  Next Obligation. prove_nodup. Defined.
+  Solve All Obligations with mod_tac.
 
-  Definition t E q sp : Mod.t := Seal.sealing CRIS (SMod.to_mod sp (smod E q)).
-End SpinLockA. End SpinLockA.
+  Definition t E sp : Mod.t := SMod.to_mod sp (smod E).
+End LockA. End LockA.
