spinlock_na/MainI.v
@@ -1,5 +1,5 @@
 Require Import CRIS.
-From CRIS.spinlock_na Require Import Header.
+Require Import LockHeader.
 Require Import ImpPrelude SchHeader MemHeader.
 
 (* Implementation of an example user module that uses spinlock library *)
@@ -9,8 +9,8 @@ Require Import ImpPrelude SchHeader MemHeader.
   3) initial state (via Any.t)
 *)
 Module SpinLockMainI. Section SpinLockMainI.
-  Context `{Σ: GRA}.
-                        
+  Context `{!crisG Γ Σ α β τ _S _I, !concGS, !memGS, !schGS, !spinlockG}.
+
   Definition scopes : list string := [].
 
   Definition main : Any.t → itree crisE Any.t :=
@@ -39,17 +39,17 @@ Module SpinLockMainI. Section SpinLockMainI.
       𝒴;;; '_ : val <- ccallU SpinLockHdr.release [Vptr l];;
       𝒴;;; Ret Vundef.
 
-  Definition fnsems : fnsems_type :=
-    [(None, (false, wmask_all, scopes, (None, main)));
-     (Some SpinLockMainHdr.incr, (false, wmask_all, scopes, (None, cfunU (sfunU incr))))].
+  Definition fnsems : fnsemmap :=
+    {[None := Some (msk_real (msk_scp scopes msk_true), (None, main));
+      Some SpinLockMainHdr.incr :=
+        Some (msk_real (msk_scp scopes msk_true), (None, cfunU (sfunU incr)))]}.
 
   Program Definition smod : SMod.t := {|
     SMod.scopes := scopes;
     SMod.fnsems := fnsems;
-    SMod.initial_st := []
+    SMod.initial_st := ∅
   |}.
-  Solve All Obligations with prove_scope.
-  Next Obligation. prove_nodup. Defined.
+  Solve All Obligations with mod_tac.
 
-  Definition t : Mod.t := Seal.sealing CRIS (SMod.to_mod sp_none smod).
+  Definition t : Mod.t := SMod.to_mod ∅ smod.
 End SpinLockMainI. End SpinLockMainI.
