spinlock_na/MainIA.v
@@ -1,237 +1,211 @@
 Require Import CRIS.
-From CRIS.spinlock_na Require Import Header MainI MainA LockI LockA.
+Require Import LockHeader MainI MainA LockI LockA.
 Require Import ImpPrelude.
-Require Import SchHeader SchA MemA SchTactics.
+Require Import SchHeader SchA MemA SchTactics MemTactics.
 From iris Require Import frac_auth numbers.
 
 Module MainIA. Section MainIA.
-  Import LockAS MainAS.
-  Context `{_crisG: !crisG Γ Σ α β τ _S _I}.
-  Context `{_memG: !memG}.
-  Context `{_schG: !schG}.
-  Context `{_spinlockG: !spinlockG}.
-  Context `{_spinlockmainG: !spinlockmainG}.
+  Context `{!crisG Γ Σ α β τ _S _I, !concGS, !memGS, !schGS, !spinlockG, !spinlockmainG}.
+  Import LockA MainA.
 
-  Context (E : coPset) (q: Qp).
-  Context (sp_s sp_t: sp_type). (* sps of lock/sch/mem *)
-  Context (sp_user_s sp_user_t: spl_type).
-  Context (SchInSp_s : sp_incl (SchAS.sp sp_user_s E q) sp_s).
-  Context (SchInSp_t : sp_incl (SchAS.sp sp_user_t E (q / 2)) sp_t).
-  Context (MainInSp : spl_sub (MainAS.sp E q) sp_user_s).
+  Context (N : namespace).
+  Context (sp_s sp_t sp_user_s sp_user_t : specmap). (* sps of lock/sch/mem *)
+  Context (SchInSp_s : (SchA.sp sp_user_s (↑N)) ⊆ sp_s).
+  Context (SchInSp_t : (SchA.sp sp_user_t (↑N)) ⊆ sp_t).
+  Context (MainInSp : (MainA.sp (↑N)) ⊆ sp_user_s).
 
-  Local Definition MemA := MemA.t.
-  Local Definition SpinLockA := (SpinLockA.t E (q / 2) sp_t).
-  Local Definition SpinLockMainA := (SpinLockMainA.t E q sp_s).
+  Local Definition MemA := MemA.t sp_s.
+  Local Definition SpinLockA := (LockA.t (↑N) sp_t).
+  Local Definition SpinLockMainA := (MainA.t N sp_s).
   Local Definition SpinLockMainI := (SpinLockMainI.t).
   Local Definition IstFull := (IstProd (IstSB SpinLockMainA.(Mod.scopes) IstTrue) IstEq).
   Local Notation MA := (SpinLockMainA ★ (SpinLockA ★ MemA)).
   Local Notation MI := (SpinLockMainI ★ (SpinLockA ★ MemA)).
 
-  Definition init_cond := MainAS.init_cond E q.
-
-  Lemma incr_simF :
-    ISim.sim_fun open MA MI init_cond IstFull (Some SpinLockMainHdr.incr).
+  Lemma incr_simF : ISim.sim_fun open MA MI IstFull (Some SpinLockMainHdr.incr).
   Proof using SchInSp_s SchInSp_t MainInSp.
-    init_simF.
+    iStartSim.
     (* process src precondition *)
-    steps_l. iDestruct "ASM" as "[TID [[-> [%γ_l [#I F]]] ->]]". hss.
-    destruct _q5 as [blk_l ofs_l], _q6 as [blk_v ofs_v].
-    rename _q4 into γ_v, _q1 into tid.
+    steps_l. destruct _q as [[stid mtid] [[[blk_l ofs_l] [blk_v ofs_v]] γ_v]]. rename _q0 into varg.
+    iDestruct "ASM" as "[TID [-> [-> [%γ_l [#Lock Tkn]]]]]".
+    hss_l; hss_r. steps_l; steps_r. hss_l; hss_r. steps_l; steps_r.
+
     (* main code *)
-    steps_l. hss. steps_l. rewrite /SpinLockMainA.incr. steps_l.
-    steps_r. hss. steps_r. rewrite /SpinLockMainI.incr. steps_r.
+    rewrite /incr /SpinLockMainI.incr. steps_l. steps_r.
     (* tgt yields *)
-    sch_yield_ir.
-    steps_r.
+    sch_yield_ir "IST" "TID". steps_r.
+    sch_yield_ir "IST" "TID". steps_r.
+
     (* tgt inline - lock acquire *)
-    sch_yield_ir.
-    steps_r. inline_r. force_r (tid, (γ_l, Vptr (blk_l, ofs_l), existT 0 (lock_P (blk_v, ofs_v) γ_v))).
+    steps_r. inline_r.
+    force_r (_, _, (γ_l, Vptr (blk_l, ofs_l), existT 0 (lock_P (blk_v, ofs_v) γ_v))).
     steps_r. forces_r.
-    rewrite -{1}(Qp.div_2 q); iPoseProof (SchAS.tid_user_split with "TID") as "[TID1 ITD2]".
-    iFrame. iSplit; eauto. hss. steps_r.
-    sch_yield_ii; [erewrite Qp.div_2; et|].
+    (* rewrite -{1}(Qp.div_2 q); iPoseProof (SchAS.tid_user_split with "TID") as "[TID1 ITD2]". *)
+    iFrame "TID Lock". iSplit; eauto. steps_r. hss_r. steps_r.
+    sch_yield_ii "IST".
 
     (* (* success case *) *)
-    steps_r. iDestruct "GRT" as "[TID' [[-> [TKN P]] _]]". hss. steps_r.
-    iPoseProof (SchAS.tid_user_merge with "[TID TID']") as "TID"; iFrame; rewrite Qp.div_2.
+    steps_r. iDestruct "GRT" as "[TID [<- [_ [TKN P]]]]". hss_r. steps_r.
+    sch_yield_ir "IST" "TID".
+
     (* tgt yield *)
-    sch_yield_ir.
-    do 2 rewrite sl_red. iDestruct "P" as "(%x & PT & P)".
-    (* tgt inline - mem load *)
-    steps_r. inline_r. steps_r.
-    force_r (blk_v, ofs_v, 1%Qp, Vint x). forces_r.
-    iSplitL "PT"; iFrame; eauto.
-    steps_r. iDestruct "GRT" as "[[PT %] %]"; subst. hss. steps_r.
-    (* tgt yield *)
-    do 2 (sch_yield_ir).
-    (* tgt inline - mem store *)
-    steps_r. inline_r. steps_r.
-    force_r (blk_v, ofs_v, _, Vint (x + 1)). forces_r.
-    iSplitL "PT"; iFrame; et.
-    steps_r. iDestruct "GRT" as "[[PT %] %]"; subst. hss_r; steps_r.
-    sch_yield_ir.
-    iCombine "P F" as "C". iMod (own_update with "C") as "[F C]".
+    solve_base_sl_red. iDestruct "P" as "[%x [PT P]]".
+    steps_r. load_r "PT". steps_r. hss_r. steps_r.
+    sch_yield_ir "IST" "TID". steps_r.
+    sch_yield_ir "IST" "TID". steps_r.
+
+    store_r "PT". steps_r. hss_r. steps_r.
+    sch_yield_ir "IST" "TID". steps_r.
+
+    iCombine "P Tkn" as "C". iMod (own_update with "C") as "[F C]".
     { apply frac_auth_update, (Z_local_update _ _ (x + 1) 1); lia. }
+    inline_r. steps_r.
+    force_r (_, _, (γ_l, Vptr (blk_l, ofs_l), existT 0 (lock_P (blk_v, ofs_v) γ_v))). forces_r.
+    iSplitL "TID F PT TKN".
+    { solve_base_sl_red. iFrame. iSplit; eauto. }
+    steps_r. hss_r; steps_r.
+    sch_yield_ii "IST". steps_r.
+    
     (* tgt inline - lock acquire - restore lock protected proposition *)
-    steps_r. inline_r. steps_r. force_r (tid, (γ_l, Vptr (blk_l, ofs_l), existT 0 (lock_P (blk_v, ofs_v) γ_v))).
-    rewrite -{1}(Qp.div_2 q); iPoseProof (SchAS.tid_user_split with "TID") as "[TID1 ITD2]".
-    forces_r. iSplitL "TID1 F PT TKN".
-    { do 2 rewrite sl_red. rewrite /lock_P; ss.
-      iFrame "TID1". iSplit; iFrame; eauto.
-    }
-    steps_r. hss. steps_r.
-    (* tgt yield *)
-    sch_yield_ii; [erewrite Qp.div_2; et|].
-    steps_r. iDestruct "GRT" as "[TID' [-> _]]". hss. steps_r.
-    iPoseProof (SchAS.tid_user_merge with "[TID TID']") as "TID"; iFrame; rewrite Qp.div_2.
-    sch_yield_ir.
+    iDestruct "GRT" as "[TID [<- _]]". hss_r. steps_r.
+    (* iPoseProof (SchAS.tid_user_merge with "[TID TID']") as "TID"; iFrame; rewrite Qp.div_2. *)
+    sch_yield_ir "IST" "TID".
     (* src yield *)
     sch_yield_l. steps_l. forces_l. iFrame; iSplit; eauto.
     (* both terminate *)
     step. iFrame. eauto.
   (*SLOW*)Qed.
 
-  Lemma main_simF :
-    ISim.sim_fun open MA MI init_cond IstFull None.
+  Lemma main_simF : ISim.sim_fun open MA MI IstFull None.
   Proof using SchInSp_s SchInSp_t MainInSp.
-    init_simF.
-    rewrite /Sch.spawn /Sch.join.
+    iStartSim. steps_l. destruct _q as [[stid mtid] []]. iDestruct "ASM" as "[TID ->]".
 
-    (* establish IST *)
-    iClear "IST".
-    iAssert (IstFull [] []) as "IST".
-    { do 4 (iExists []). iPureIntro. esplits; et; ss. }
-    iRevert "IST"; iIntros "IST"; rewrite bi.intuitionistically_elim.
+    rewrite /main. steps_l.
+    steps_r. rewrite /SpinLockMainI.main. steps_r.
+    rewrite /Sch.spawn.
 
-    steps_l. steps_r.
     (* tgt yield *)
-    sch_yield_ir.
+    sch_yield_ir "IST" "TID".
 
     (* tgt inline - mem alloc - counter allocation *)
-    steps_r. inline_r. steps_r.
-    force_r 1. forces_r. iSplit; eauto.
-    steps_r. iDestruct "GRT" as "[[%blk [% [GRT _]]] %]"; subst. hss. steps_r.
-    sch_yield_ir.
+    steps_r.
+    iApply wsim_mem_alloc; ss. iIntros (blk) "[↦ _]". steps_r. hss_r. steps_r.
+    sch_yield_ir "IST" "TID".
+
     (* tgt inline - mem store - counter initialization *)
-    steps_r. inline_r. steps_r.
-    force_r (blk, 0%Z, _, Vint 0). forces_r.
-    iFrame; iSplit; eauto.
-    steps_r. iDestruct "GRT" as "[[PT %] %]"; subst. hss. steps_r.
-    sch_yield_ir.
+    steps_r.
+    iApply (wsim_mem_store with "[↦]"); ss. iIntros"↦". steps_r. hss_r. steps_r.
+    sch_yield_ir "IST" "TID".
+
     (* create lock-guarded proposition *)
-    iMod (own_alloc (●F 0%Z ⋅ ◯F{1} 0%Z)) as "(%γ & B & W)".
-    { eapply frac_auth_valid; ss. }
+    iMod (own_alloc (●F 0%Z ⋅ ◯F{1} 0%Z)) as "[%γ [B W]]". { eapply frac_auth_valid; ss. }
+
     (* tgt inline - newlock *)
-    steps_r. inline_r. steps_r.
-    force_r (0, existT 0 (lock_P (blk, 0%Z) γ)). forces_r.
-    rewrite -{1}(Qp.div_2 q); iPoseProof (SchAS.tid_user_split with "TID") as "[TID1 ITD2]".
-    iSplitL "TID1 B PT"; eauto.
-    { iFrame; rewrite sl_red; iSplit; eauto. iFrame. }
-    steps_r. hss. steps_r.
+    steps_r. inline_r. force_r (stid, mtid, existT 0 (lock_P (blk, 0%Z) γ)). forces_r.
+    iSplitL "TID B ↦"; eauto.
+    { iFrame. solve_base_sl_red. iFrame. done. }
+    steps_r. hss_r. steps_r.
+
     (* src/tgt yields *)
-    sch_yield_ii; [erewrite Qp.div_2; et|].
-    steps_r. iDestruct "GRT" as "[TID' [[%val [%γ_l [-> #I]]] %EQ]]".
-    hss. steps_r.
-    iPoseProof (SchAS.tid_user_merge with "[TID TID']") as "TID"; iFrame; rewrite Qp.div_2.
-    sch_yield_ir.
-    iPoseProof "I" as "[%bofs_l [-> _]]".
+    sch_yield_ii "IST".
+    steps_r. iDestruct "GRT" as "[TID [-> [%val [%γl [-> [%bofs_l [-> #Lock]]]]]]]".
+    hss_r. steps_r.
+    sch_yield_ir "IST" "TID".
+
+    (* iPoseProof "I" as "[%bofs_l [-> _]]". *)
     sch_yield_l. steps_l. force_l (Vptr bofs_l, Vptr (blk, 0%Z)). steps_l. sch_yield_l.
     (* create preconditions of incr *)
     iDestruct "W" as "[W1 W2]".
 
     (* spawn thread 1 - incr *)
-    steps_l. steps_r. force_l (_,_,_). forces_l. iSplitL "W1 TID".
-    { iExists (_,_). iSplit; et. iFrame. iExists _, _, _. iSplit.
-      - iPureIntro; esplits; et. r; eauto using incr_spawnable.
-      - iFrame; et.
+    steps_l. simpl_sp. steps_r. force_l (_,_). forces_l. iSplitL "W1".
+    { iExists _, _, _. iSplit; et. iSplitR.
+      - iExists _; iSplit; [iPureIntro; simpl_sp|]; ss. iApply incr_spawnable.
+      - iFrame "W1"; eauto. repeat iSplit; eauto. iExists _; iFrame "Lock"; auto.
     }
-    call "IST".
-    steps_l. iDestruct "ASM" as "[% [-> [TID [% [[-> ->] TKN1]]]]]".
-    rename _q0 into tid1.
-    steps_r. hss. steps_r.
-    sch_yield_ir. sch_yield_l.
+    call "IST". clear_st; iIntros (ret st_src st_tgt) "IST".
+    steps_l. iDestruct "ASM" as "[% [[-> ->] TKN1]]". 
+    steps_r. hss_r. steps_r. hss_l. steps_l.
+    sch_yield_ir "IST" "TID". sch_yield_l.
 
     (* spawn thread 2 - incr *)
-    steps_l. steps_r. force_l (_,_,_). forces_l. iSplitL "W2 TID".
-    { iExists (_,_). iSplit; et. iFrame. iExists _, _, _. iSplit.
-      - iPureIntro; esplits; et. r; eauto using incr_spawnable.
-      - iFrame; et.
+    steps_l. simpl_sp. steps_r. force_l (_,_). forces_l. iSplitL "W2".
+    { iExists _, _, _. iSplit; et. iSplitR.
+      - iExists _; iSplit; [iPureIntro; simpl_sp|]; ss. iApply incr_spawnable.
+      - iFrame "W2"; eauto. repeat iSplit; eauto. iExists _; iFrame "Lock"; auto.
     }
-    call "IST".
-    steps_l. iDestruct "ASM" as "[% [-> [TID [% [[-> ->] TKN2]]]]]". hss.
-    rename _q0 into tid2.
-    steps_r. hss. steps_r.
-    sch_yield_ir. sch_yield_l.
+    call "IST". clear_st; iIntros (ret st_src st_tgt) "IST".
+    steps_l. iDestruct "ASM" as "[% [[-> ->] TKN2]]". 
+    steps_r. hss_r. steps_r. hss_l. steps_l.
+    sch_yield_ir "IST" "TID". sch_yield_l.
 
     (* join thread 1 - incr *)
-    steps_l. steps_r.  force_l (_,_,_). forces_l. iSplitL "TID TKN1".
-    { iExists _. do 2 (iSplit; et). iFrame. }
-    call "IST".
-    steps_l. iDestruct "ASM" as "[% [-> [% [% [[-> ->] [TID W1]]]]]]".
-    hss. rename _q1 into vret.
-    steps_r. hss. steps_r.
-    sch_yield_ir. sch_yield_l.
+    rewrite /Sch.join.
+    steps_l. steps_r. simpl_sp. force_l (_,_,_). forces_l. iSplitL "TKN1 TID".
+    { iFrame. eauto. }
+    call "IST". clear_st; iIntros (ret st_src st_tgt) "IST".
+    steps_l. steps_r. iDestruct "ASM" as "[TID [% [% [[-> ->] W1]]]]". solve_base_sl_red.
+    hss_l; hss_r. steps_l; steps_r.
+    sch_yield_ir "IST" "TID". sch_yield_l. steps_r. steps_l. simpl_sp.
 
     (* join thread 2 - incr *)
-    steps_l. steps_r.  force_l (_,_,_). forces_l. iSplitL "TID TKN2".
-    { iExists _. do 2 (iSplit; et). iFrame. }
-    call "IST".
-    steps_l. iDestruct "ASM" as "[% [-> [% [% [[-> ->] [TID W2]]]]]]".
-    hss. rename _q1 into vret0.
-    steps_r. hss. steps_r.
-    sch_yield_ir.
+    force_l (stid, mtid, _). forces_l. iSplitL "TID TKN2".
+    { iFrame; eauto. }
+    call "IST". clear_st; iIntros (ret st_src st_tgt) "IST".
+    steps_l. iDestruct "ASM" as "[TID [% [% [[-> ->] W2]]]]". solve_base_sl_red. steps_r.
+    hss_l; hss_r. steps_l; steps_r.
+    sch_yield_ir "IST" "TID". steps_r.
 
     (* tgt inline - lock acquire *)
-    steps_r. inline_r. steps_r.
-    force_r (_, (γ_l, Vptr bofs_l, existT 0 (lock_P (blk, 0%Z) γ))). forces_r.
-    rewrite -{1}(Qp.div_2 q); iPoseProof (SchAS.tid_user_split with "TID") as "[TID1 ITD2]".
-    iFrame. iSplit; eauto.
-    steps_r. hss. steps_r.
-    sch_yield_ii; [erewrite Qp.div_2; et|].
-    steps_r. iDestruct "GRT" as "[TID' [[-> [TKN P]] _]]". hss. steps_r.
-    do 3 rewrite sl_red. iCombine "W1 W2" as "W".
-    iDestruct "P" as "(%x & PT & B)".
+    inline_r. steps_r.
+    force_r (_, _, (γl, Vptr bofs_l, existT 0 (lock_P (blk, 0%Z) γ))). forces_r.
+    iFrame "TID"; iSplitR.
+    { repeat iSplit; eauto. iFrame "Lock"; auto. }
+    steps_r. hss_r. steps_r.
+    sch_yield_ii "IST". steps_r.
+    iDestruct "GRT" as "[TID [<- [_ [TKN P]]]]". hss_r. steps_r.
+    sch_yield_ir "IST" "TID". steps_r.
+    iCombine "W1 W2" as "W". solve_base_sl_red.
+    iDestruct "P" as "[%x [PT B]]".
     iCombine "B W" gives %WF%frac_auth_agree. inv WF.
-    iPoseProof (SchAS.tid_user_merge with "[TID TID']") as "TID"; iFrame; rewrite Qp.div_2.
-    sch_yield_ir.
+
     (* tgt inline - mem load *)
-    steps_r. inline_r. steps_r.
-    force_r (blk, 0%Z, 1%Qp, Vint 2%Z). forces_r.
-    iFrame "PT". iSplit; et.
-    steps_r. iDestruct "GRT" as "[[PT %] %]"; subst. hss. steps_r.
+    load_r "PT". steps_r. hss_r. steps_r.
+
     (* tgt yield *)
-    do 2 (sch_yield_ir).
+    sch_yield_ir "IST" "TID". steps_r.
+    sch_yield_ir "IST" "TID". steps_r.
+
     (* tgt inline - lock release *)
-    steps_r. inline_r. steps_r.
-    force_r (_, (γ_l, Vptr bofs_l, existT 0 (lock_P (blk, 0%Z) γ))). forces_r.
-    rewrite -{1}(Qp.div_2 q); iPoseProof (SchAS.tid_user_split with "TID") as "[TID1 ITD2]".
-    iSplitL "TKN TID1 B PT".
-    { iFrame. do 2 rewrite sl_red. iSplit; eauto. iFrame. iSplit; eauto. }
-    steps_r. hss. steps_r.
+    inline_r. steps_r.
+    force_r (_, _, (γl, Vptr bofs_l, existT 0 (lock_P (blk, 0%Z) γ))). forces_r.
+    iSplitL "TKN TID B PT".
+    { solve_base_sl_red. iFrame. iFrame "Lock"; iSplit; eauto. }
+    steps_r. hss_r. steps_r.
+
     (* tgt yield *)
-    sch_yield_ii; [erewrite Qp.div_2; et|].
-    steps_r. iDestruct "GRT" as "[TID' [-> _]]". hss. steps_r.
-    iPoseProof (SchAS.tid_user_merge with "[TID TID']") as "TID"; iFrame; rewrite Qp.div_2.
-    sch_yield_ir.
+    sch_yield_ii "IST". steps_r. iDestruct "GRT" as "[TID [<- _]]". hss_r. steps_r.
+    sch_yield_ir "IST" "TID".
+
     (* both output - counter value *)
     sch_yield_l. step.
     steps_l. steps_r.
-    sch_yield_ir.
-    sch_yield_l. 
+    sch_yield_ir "IST" "TID". sch_yield_l.
     (* terminate both *)
-    step. iSplit; eauto.
+    forces_l. iFrame; iSplit; first eauto. step. iSplit; eauto.
   (*SLOW*)Qed.
 
-  Lemma sim : ISim.t open MA MI init_cond IstFull.
+  Lemma sim : ISim.t open MA MI emp%I IstFull.
   Proof.
     init_sim.
     { eapply main_simF. }
     { eapply incr_simF. }
+    { iIntros "_"; repeat iExists _; repeat iSplit; eauto. }
   Qed.
 
   Definition ctxr :
     ctx_refines
-    ((SpinLockMainA.t E q sp_s) ★ ((SpinLockA.t E (q/2) sp_t) ★ MemA.t), init_cond)
-    ((SpinLockMainI.t)          ★ ((SpinLockA.t E (q/2) sp_t) ★ MemA.t), emp%I).
+      ((MainA.t N sp_s)  ★ ((LockA.t (↑N) sp_t) ★ MemA.t sp_s), emp%I)
+      ((SpinLockMainI.t) ★ ((LockA.t (↑N) sp_t) ★ MemA.t sp_s), emp%I).
   Proof. eapply main_adequacy, sim. Qed.
 End MainIA. End MainIA.
